UnionFind alloc cleanup

UnionFind.v
@@ -142,36 +142,32 @@ Proof.
 Qed.
   
 Hint Resolve refl_δ.
+Check alloc.
+Definition init_cell {n:nat} (i:nat) (pf:i<n) : hpred (cell n) :=
+  (fun x h => x = mkCell n 0 (of_nat_lt pf)).
+Lemma prec_init : forall n i pf, precise_pred (@init_cell n i pf).
+Proof. intros; red; intros. inversion H. constructor. Qed.
+Hint Resolve prec_init.
+Lemma stable_init : forall n i pf, stable (@init_cell n i pf) local_imm.
+Proof. intros. red; intros. inversion H0; subst. auto. Qed.
+Hint Resolve stable_init.
 
 Program Definition alloc_uf {Γ} (n:nat) : rgref Γ (ref{uf n|φ n}[δ n, δ n]) Γ :=
   (*arr <- indep_array n (fun i pf => Alloc (mkCell n 0 (of_nat_lt pf)));
   Alloc arr.*)
-  indep_array_conv_alloc n (fun i pf => Alloc (mkCell n 0 (of_nat_lt pf))) _ _.
-Next Obligation. red; intros. exact (H = mkCell n 0 (of_nat_lt pf)). Defined.
-Next Obligation. exact local_imm. Defined.
-Next Obligation. exact local_imm. Defined.
-Next Obligation. unfold alloc_uf_obligation_1. unfold alloc_uf_obligation_2.
-  red; intros. inversion H0; subst. rewrite <- H1. reflexivity. Qed.
-Next Obligation. intuition. Qed.
-Next Obligation. unfold alloc_uf_obligation_1. red. intros. subst; auto. Qed.
-Next Obligation. unfold alloc_uf_obligation_2. red. intros. inversion H1. subst. constructor. Qed.
-Next Obligation. unfold alloc_uf_obligation_3. red; intros. inversion H1; subst. constructor. Qed.
-Next Obligation. 
-  unfold alloc_uf_obligation_1 in *.
-  unfold alloc_uf_obligation_2 in *.
-  unfold alloc_uf_obligation_3 in *.
-  eapply convert; eauto.
-Defined.
+  (*indep_array_conv_alloc n (fun i pf => Alloc (mkCell n 0 (of_nat_lt pf))) _ _.*)
+  indep_array_conv_alloc n (fun i pf => alloc (init_cell i pf) local_imm local_imm 
+                                              (mkCell n 0 (of_nat_lt pf)) _ _ _ _ _ _
+                           ) _ _.
+Next Obligation. constructor. Qed.
+Next Obligation. eapply convert; eauto. Defined.
 Next Obligation.
   (* Prove φ of the initial array.  Need the array allocation to expose some summary of the
      initialization process, something like making the result of the allocation function
      depend on the index, together with a conversion that weakens that result (like loosening
      a refinement that the parent pointer is the cell number initially) and some way to
      stitch those together for an array-wide refinement... *)
-  unfold alloc_uf_obligation_1 in *.
-  unfold alloc_uf_obligation_2 in *.
-  unfold alloc_uf_obligation_3 in *.
-  unfold alloc_uf_obligation_10 in *.
+  unfold alloc_uf_obligation_7 in *.
   constructor. intros.
   constructor.
   assert (exists i0, exists (pf:i0 < n), i = of_nat_lt pf).
